Quicksort/Partition/Hoare/Basic.lean
@@ -3,21 +3,21 @@ import Quicksort.Partition.Hoare.Eager.Basic
 
 open Vector
 
-def Partition.hoare [Ord α] (arr : Vector α n) (left : Nat)  (right : Nat) (hlr : left < right) (hr : right < n) : {x : Partition α n // (left < x.i') ∧ (x.j' < right)} :=
+def Partition.hoare (arr : Vector α n) (left : Nat)  (right : Nat) (hlr : left < right) (hr : right < n) (lt : α → α → Bool := by exact (· < ·)): {x : Partition α n // (left < x.i') ∧ (x.j' < right)} :=
   have hl : left < n := by omega
 
   let mid := left + ((right - left)/2)
   have hm : mid < n := by omega
   let arr_ := arr
-    |> (maybeSwap · ⟨left, hl⟩ ⟨mid, hm⟩)
-    |> (maybeSwap · ⟨left, hl⟩ ⟨right, hr⟩)
-    |> (maybeSwap · ⟨mid, hm⟩ ⟨right, hr⟩)
+    |> (maybeSwap (lt := lt) · ⟨left, hl⟩ ⟨mid, hm⟩)
+    |> (maybeSwap (lt := lt) · ⟨left, hl⟩ ⟨right, hr⟩)
+    |> (maybeSwap (lt := lt) · ⟨mid, hm⟩ ⟨right, hr⟩)
 
   let pivot := arr_[mid]
 
   if hmo3sortd : ¬lt pivot arr_[left] ∧ ¬lt arr_[right] pivot then
-    hoare.classic.loop left right hr hl pivot arr_ (left + 1) (right - 1) Nat.le.refl (by omega) (by omega) hmo3sortd.left hmo3sortd.right
+    hoare.classic.loop (lt := lt) left right hr hl pivot arr_ (left + 1) (right - 1) Nat.le.refl (by omega) (by omega) hmo3sortd.left hmo3sortd.right
   else
-    have := hoare.eager.loop left right hr pivot arr_ (left + 1) (right - 1) (by omega) (by omega) (by omega)
+    have := hoare.eager.loop (lt := lt) left right hr pivot arr_ (left + 1) (right - 1) (by omega) (by omega) (by omega)
     |> (Inhabited.mk ·)
     panic! "non-asymmetric or non-transitive comparitor. falling back to eager version of hoare partition scheme"
