Quicksort/Partition/Init/Basic.lean
@@ -1,11 +1,11 @@
-def lt [Ord α] (x y : α) : Bool :=
-  match compare x y with
-  | .lt => true
-  | _ => false
+-- def lt (lt : α → α → Bool := by exact (· < ·)) (x y : α) : Bool :=
+--   match compare x y with
+--   | .lt => true
+--   | _ => false
 
 -- abbrev lt [Ord α] (x y : α) := compare x y |>.isLT
 
-def Vector.maybeSwap [Ord α] (as : Vector α n) (low high : Fin n) : Vector α n :=
+def Vector.maybeSwap (lt : α → α → Bool := by exact (· < ·)) (as : Vector α n) (low high : Fin n) : Vector α n :=
   if lt as[high] as[low] then
     as.swap low high
   else
@@ -18,7 +18,7 @@ structure Partition (α: Type u) (n : Nat)  where
   i' : Nat
   deriving Repr, Nonempty, Inhabited
 
-abbrev Partition.Scheme α :=  [Ord α] → {n : Nat} → Vector α n → (left right : Nat) → left < right → right < n →  { x : Partition α n  // left < x.i' ∧ x.j' < right }
+abbrev Partition.Scheme α :=  {n : Nat} → Vector α n → (left right : Nat) → left < right → right < n → (lt : α → α → Bool := by exact (· < ·)) →  { x : Partition α n  // left < x.i' ∧ x.j' < right }
 
 -- private def dbg {α : Type u} [ToString α] (a : α) (s : String)  : α :=
 --   dbgTrace s!"{s}" (fun _ => a)
