Quicksort/Partition/Lemmas.lean
@@ -6,15 +6,15 @@ import Quicksort.Partition.Basic
 open Vector
 
 namespace Partition
-variable [Ord α]
+variable (lt : α → α → Bool := by exact (· < ·))
 
--- private class LT_Asymm (α : Type u) [Ord α] : Prop where
--- private class LE_Trans (α : Type u) [Ord α] : Prop where
+-- private class LT_Asymm (α : Type u) (lt : α → α → Bool := by exact (· < ·)) : Prop where
+-- private class LE_Trans (α : Type u) (lt : α → α → Bool := by exact (· < ·)) : Prop where
 
 -- -- variable (le_trans : ∀ {x y z : α}, ¬lt y x → ¬lt z y → ¬lt z x)
 -- -- variable (lt_asymm : ∀ {x y : α}, lt x y → ¬lt y x)
 
-class StrictOrder (α : Type u) [Ord α]  : Prop where
+class StrictOrder (α : Type u) (lt : α → α → Bool)  : Prop where
   lt_asymm : ∀ {x y : α}, lt x y → ¬lt y x
   le_trans : ∀ {x y z : α}, ¬lt y x → ¬lt z y → ¬lt z x
 
@@ -22,21 +22,21 @@ export StrictOrder (lt_asymm le_trans)
 
 
 class LawfulScheme (part : Partition.Scheme α) : Prop where
-  partitionBounds : (part as left right hlr hr).val.j' < (part as left right hlr hr).val.i'
-  permStabilizing : PermStabilizing' left right (part as left right hlr hr).val.arr' as
-  sorting [StrictOrder α] (as : Vector α n) (hlr : left < right) (hr : right < n) : ∃ (pivot : α), IsPartitioned left right pivot (part as left right hlr hr).val
+  partitionBounds : (part (lt := lt) as left right hlr hr).val.j' < (part (lt := lt) as left right hlr hr).val.i'
+  permStabilizing : PermStabilizing' left right (part (lt := lt) as left right hlr hr).val.arr' as
+  sorting [StrictOrder α lt] (as : Vector α n) (hlr : left < right) (hr : right < n) : ∃ (pivot : α), IsPartitioned (lt := lt) left right pivot (part (lt := lt) as left right hlr hr).val
 
-instance instLawfulHoareScheme : LawfulScheme (α := α) hoare where
-  partitionBounds := hoare.partition_bounds
-  permStabilizing := hoare.permStabilizing
-  sorting _ _ _ := hoare.sorted lt_asymm le_trans
+instance instLawfulHoareScheme : LawfulScheme (lt := lt) (α := α) (part := @hoare α) where
+  partitionBounds := hoare.partition_bounds (lt := lt)
+  permStabilizing := hoare.permStabilizing (lt := lt)
+  sorting _ _ _ := hoare.sorted lt_asymm le_trans (lt := lt)
 
-instance instLawfulLomutoScheme : LawfulScheme (α := α) lomuto where
-  partitionBounds := lomuto.partition_bounds
-  permStabilizing := lomuto.permStabilizing
-  sorting _ _ _ := lomuto.sorted lt_asymm
+instance instLawfulLomutoScheme : LawfulScheme (lt := lt) (α := α) (part := @lomuto α) where
+  partitionBounds := lomuto.partition_bounds (lt := lt)
+  permStabilizing := lomuto.permStabilizing (lt := lt)
+  sorting _ _ _ := lomuto.sorted lt_asymm (lt := lt)
 
-instance  instLawfulDefaultScheme : LawfulScheme (α := α) (@default _ _) := by
+instance  instLawfulDefaultScheme : LawfulScheme (lt := lt) (α := α) (@default _ _) := by
   simp only [default]; first
-  | exact instLawfulHoareScheme
-  | exact instLawfulLomutoScheme
+  | exact instLawfulHoareScheme (lt := lt)
+  | exact instLawfulLomutoScheme (lt := lt)
