Quicksort/Lemmas.lean
@@ -4,14 +4,15 @@ import Quicksort.Basic
 open Partition
 open Array
 
-variable [Ord α]
+variable (lt : α → α → Bool := by exact (· < ·))
 
-theorem qs.strict.permStabilizing [LawfulScheme part] {as : Vector α n} {left right : Nat} {hsize' : right ≤ n - 1} : Vector.PermStabilizing' left right (qs.strict part as left right hsize') as := by
-  induction as, left, right, hsize' using qs.strict.induct (part := part) with
+
+theorem qs.strict.permStabilizing [LawfulScheme (lt := lt) @part] {as : Vector α n} {left right : Nat} {hsize' : right ≤ n - 1} : Vector.PermStabilizing' left right (qs.strict (lt := lt) @part as left right hsize') as := by
+  induction as, left, right, hsize' using qs.strict.induct (lt := lt) (part := @part) with
   | case1 as left right hsize' hlr as' j' i' hli hjr heq as'' ih1 _ih1 ih2 =>
     unfold qs.strict; simp [*]
 
-    have ih0 := heq ▸ LawfulScheme.permStabilizing (part := part)
+    have ih0 := heq ▸ LawfulScheme.permStabilizing (part := @part)
     replace ih1 : Vector.PermStabilizing' left right .. := ih1.mono (by omega) (by omega)
     replace ih2 : Vector.PermStabilizing' left right .. := ih2.mono (by omega) (by omega)
 
@@ -20,43 +21,43 @@ theorem qs.strict.permStabilizing [LawfulScheme part] {as : Vector α n} {left r
     unfold qs.strict; simp [*]
     apply Vector.PermStabilizing'.refl
 
-theorem qs.perm' [LawfulScheme part] {as : Array α} {left : Nat} {right : Nat}  : (qs as left right part).Perm as := by
+theorem qs.perm' [LawfulScheme (lt := lt) @part] {as : Array α} {left : Nat} {right : Nat}  : (qs (lt := lt) as left right @part).Perm as := by
   simp only [qs]; split
   any_goals simp only [panicWithPosWithDecl, panic, panicCore, *]
   all_goals
-  have := qs.strict.permStabilizing (part := part) (as := Vector.mk as rfl) (left := left) (hsize' := by solve_by_elim) |>.1
+  have := qs.strict.permStabilizing  (lt := lt) (part := @part) (as := Vector.mk as rfl) (left := left) (hsize' := by solve_by_elim) |>.1
   grind [Vector.Perm]
 
 
-theorem qs.perm {as : Array α} : (qs as).Perm as := qs.perm'
+theorem qs.perm {as : Array α} : (qs (lt := lt) as).Perm as := qs.perm' (lt := lt)
 
 
 @[simp]
-theorem qs.qs_size [LawfulScheme part] {as : Array α} :
-    (qs as left right part).size = as.size := qs.perm'.size_eq
+theorem qs.qs_size [LawfulScheme (lt := lt) @part] {as : Array α} :
+    (qs (lt := lt) as left right @part).size = as.size := (qs.perm' (lt := lt)).size_eq
 
 
-theorem qs.strict.monotonic [StrictOrder α] [LawfulScheme part] {as : Vector α n} {hsize' : right ≤ n - 1} : let q := (qs.strict part as left right hsize'); ∀ (i j : Fin n), (left ≤ i) → (i < j) → (j ≤ right) → ¬lt q[j] q[i] := by
-  induction as, left, right, hsize' using qs.strict.induct (part := part) with
+theorem qs.strict.monotonic [StrictOrder (lt := lt) α] [LawfulScheme (lt := lt) @part] {as : Vector α n} {hsize' : right ≤ n - 1} : let q := (qs.strict (lt := lt) @part as left right hsize'); ∀ (i j : Fin n), (left ≤ i) → (i < j) → (j ≤ right) → ¬lt q[j] q[i] := by
+  induction as, left, right, hsize' using qs.strict.induct (lt := lt) (part := @part) with
   | case1 as left right hsize' hlr as' j' i' hli' hjr' heq as'' ih1 _ih1 ih2 =>
     unfold qs.strict; simp only [↓reduceDIte, hlr, heq]
 
     intro i j hli hij hjr; exact
 
     have hji' : j' < i' := by apply heq
-      ▸ LawfulScheme.partitionBounds (part := part)
-    let as''' := qs.strict part as'' i' right (by omega)
+      ▸ LawfulScheme.partitionBounds (part := @part)
+    let as''' := qs.strict (lt := lt) @part as'' i' right (by omega)
 
     if hhi : i' ≤ i then by
       apply ih2 <;> assumption
     else if hhj : j ≤ j' then by
-      rw [qs.strict.permStabilizing.2.left j (by omega), qs.strict.permStabilizing.2.left i (by omega)]
+      rw [(qs.strict.permStabilizing (lt := lt)).2.left j (by omega), (qs.strict.permStabilizing (lt := lt)).2.left i (by omega)]
       apply ih1 <;> assumption
     else by
       replace hhi : i < i' := by omega
       replace hhj : j' < j := by omega
 
-      have ⟨pivot, ih0⟩ := LawfulScheme.sorting (part := part) as hlr (by omega)
+      have ⟨pivot, ih0⟩ := LawfulScheme.sorting  (lt := lt)  (part := @part) as hlr (by omega)
       -- ih0 : Partitioned left right pivot (part as left right hlr hr).val
 
       replace ih0 :
@@ -65,26 +66,26 @@ theorem qs.strict.monotonic [StrictOrder α] [LawfulScheme part] {as : Vector α
         unfold Partition.IsPartitioned at ih0; rwa [heq] at ih0
 
       have hhh1 : ¬lt pivot as'''[i] :=
-        suffices ¬lt pivot as''[i] by rwa [qs.strict.permStabilizing.2.left i (by omega)]
+        suffices ¬lt pivot as''[i] by rwa [(qs.strict.permStabilizing (lt := lt)).2.left i (by omega)]
         if _ : i ≤ j' then by
-          apply Vector.PermStabilizing'.invariance (motive := (¬lt pivot ·)) (left := left) (hi := j' + 1) (hperm := qs.strict.permStabilizing) (h := ?_ )
+          apply Vector.PermStabilizing'.invariance (motive := (¬lt pivot ·)) (left := left) (hi := j' + 1) (hperm := (qs.strict.permStabilizing (lt := lt))) (h := ?_ )
           any_goals omega
           · intro i_ _ _
             apply ih0.left i_ <;> omega
         else by
-          rw [qs.strict.permStabilizing.2.right _ ?_]
+          rw [(qs.strict.permStabilizing (lt := lt)).2.right _ ?_]
           apply ih0.left i
           all_goals omega
 
       have hhh2 : ¬lt as'''[j] pivot :=
         if _ : i' ≤ j then by
-          apply Vector.PermStabilizing'.invariance (motive := (¬lt · pivot)) (left := i') (hi := right + 1) (hperm := qs.strict.permStabilizing) (h := ?_)
+          apply Vector.PermStabilizing'.invariance (motive := (¬lt · pivot)) (left := i') (hi := right + 1) (hperm := (qs.strict.permStabilizing (lt := lt))) (h := ?_)
           any_goals omega
           · intro j_ _ _
-            rw [qs.strict.permStabilizing.2.right j_ (by omega)]
+            rw [(qs.strict.permStabilizing (lt := lt)).2.right j_ (by omega)]
             apply ih0.right j_ <;> omega
         else by
-          rw [qs.strict.permStabilizing.2.left _ ?_, qs.strict.permStabilizing.2.right _ ?_]
+          rw [(qs.strict.permStabilizing (lt := lt)).2.left _ ?_, (qs.strict.permStabilizing (lt := lt)).2.right _ ?_]
           apply ih0.right j
           all_goals omega
       exact le_trans hhh1 hhh2
@@ -92,15 +93,15 @@ theorem qs.strict.monotonic [StrictOrder α] [LawfulScheme part] {as : Vector α
 
 -- variable (lt_asymm : ∀ {x y : α}, (lt x y) → ¬lt y x)
 
-theorem qs.monotonic' [StrictOrder α] {as : Array α} {left : Nat} {right : Nat} {part : Partition.Scheme α} [LawfulScheme part] :  let q := (qs as left right part); ∀ (i j : Fin q.size), (left ≤ i) → (i < j) → (j ≤ right) → ¬lt q[j] q[i] := by
+theorem qs.monotonic' [StrictOrder (lt := lt) α] {as : Array α} {left : Nat} {right : Nat} {part : Partition.Scheme α} [LawfulScheme (lt := lt) @part] :  let q := (qs (lt := lt) as left right @part); ∀ (i j : Fin q.size), (left ≤ i) → (i < j) → (j ≤ right) → ¬lt q[j] q[i] := by
   simp only
   intro  i j _ _ _
-  have _ : j.cast qs.qs_size ≤ as.size - 1 := by omega
+  have _ : j.cast (qs.qs_size (lt := lt)) ≤ as.size - 1 := by omega
   simp only [qs]; split
   any_goals simp only [panicWithPosWithDecl, panic, panicCore, *]
-  all_goals apply qs.strict.monotonic (i.cast qs.qs_size) (j.cast qs.qs_size) <;> assumption
+  all_goals apply qs.strict.monotonic (lt := lt) (i.cast (qs.qs_size (lt := lt))) (j.cast (qs.qs_size (lt := lt))) <;> assumption
 
-theorem qs.monotonic [StrictOrder α] {as : Array α} {part : Partition.Scheme α} [LawfulScheme part]: ∀ (i j : Fin (qs (part := part) as).size), i < j → ¬lt (qs (part := part) as)[j] (qs (part := part) as)[i] := by
+theorem qs.monotonic [StrictOrder (lt := lt) α] {as : Array α} {part : Partition.Scheme α} [LawfulScheme (lt := lt) @part]: ∀ (i j : Fin (qs (lt := lt) (part := @part) as).size), i < j → ¬lt (qs (lt := lt) (part := @part) as)[j] (qs (lt := lt) (part := @part) as)[i] := by
   intro i j h
   apply qs.monotonic'
   · omega
@@ -108,11 +109,11 @@ theorem qs.monotonic [StrictOrder α] {as : Array α} {part : Partition.Scheme �
   · have := j.2; simp only [qs.qs_size] at this; omega
 
 
-theorem qs.monotonic_with_defaults [StrictOrder α] {as : Array α} : ∀ (i j : Fin (qs as).size), i < j → ¬lt (qs as)[j] (qs as)[i] := qs.monotonic
+theorem qs.monotonic_with_defaults [StrictOrder (lt := lt) α] {as : Array α} : ∀ (i j : Fin (qs (lt := lt) as).size), i < j → ¬lt (qs (lt := lt) as)[j] (qs (lt := lt) as)[i] := qs.monotonic (lt := lt)
 
-example [StrictOrder α] {as : Array α} : let q := (qs (part := Partition.hoare) as); ∀ (i j : Fin q.size), i < j → ¬lt q[j] q[i] := qs.monotonic
-example [StrictOrder α] {as : Array α} : let q := (qs (part := Partition.lomuto) as); ∀ (i j : Fin q.size), i < j → ¬lt q[j] q[i] := qs.monotonic
+example [StrictOrder (lt := lt) α] {as : Array α} : let q := (qs (lt := lt) (part := @Partition.hoare α) as); ∀ (i j : Fin q.size), i < j → ¬lt q[j] q[i] := qs.monotonic (lt := lt)
+example [StrictOrder (lt := lt) α] {as : Array α} : let q := (qs (lt := lt) (part := @Partition.lomuto α) as); ∀ (i j : Fin q.size), i < j → ¬lt q[j] q[i] := qs.monotonic (lt := lt)
 
--- def unlawful_partition [Ord α] {n : Nat} (arr : Vector α n) (left : Nat)  (right : Nat) (hlr : left < right) (hr : right < n) : {x : Partition α n // (left < x.i') ∧ (x.j' < right)} := sorry
+-- def unlawful_partition (lt : α → α → Bool := by exact (· < ·)) {n : Nat} (arr : Vector α n) (left : Nat)  (right : Nat) (hlr : left < right) (hr : right < n) : {x : Partition α n // (left < x.i') ∧ (x.j' < right)} := sorry
 
 -- example {as : Array α} : let q := (qs (part := unlawful_partition) as); ∀ (i j : Fin q.size), i < j → ¬lt q[j] q[i] := qs.monotonic (part := unlawful_partition) -- <-- Should not work
