Quicksort/Partition/Basic.lean
@@ -1,5 +1,5 @@
 import Quicksort.Partition.Hoare.Basic
 import Quicksort.Partition.Lomuto.Basic
 
--- instance instInhabitedSchemeOfOrd [Ord α] : Inhabited (Partition.Scheme α) := ⟨Partition.lomuto⟩
-instance instInhabitedSchemeOfOrd' [Ord α] : Inhabited (Partition.Scheme α) := ⟨Partition.hoare⟩
+-- instance instInhabitedSchemeOfOrd : Inhabited (Partition.Scheme α) := ⟨@Partition.lomuto (α := α)⟩
+instance instInhabitedSchemeOfOrd' : Inhabited (Partition.Scheme α) := ⟨@Partition.hoare (α := α)⟩
