Quicksort/Partition/Hoare/Classic/Lemmas.lean
@@ -5,7 +5,8 @@ import Quicksort.Partition.Init.Lemmas
 open Vector
 
 namespace Partition
-variable [Ord α]
+variable (lt : α → α → Bool := by exact (· < ·))
+
 variable (lt_asymm : ∀ {x y : α}, lt x y → ¬lt y x)
 
 include lt_asymm in
@@ -17,8 +18,8 @@ variable (le_trans : ∀ {x y z : α}, ¬lt y x → ¬lt z y → ¬lt z x)
 
 
 theorem hoare.classic.while_i_elem_not_left_of_piv {arr : Vector α n} {harltp : ¬lt arr[right] pivot}
-  : ¬lt arr[(hoare.classic.loop.while_i left right hr pivot arr i j hjr harltp ival hii hxi).1.val] pivot := by
-  induction ival, hii, hxi using hoare.classic.loop.while_i.induct right hr pivot arr i j harltp with
+  : ¬lt arr[(hoare.classic.loop.while_i (lt := lt) left right hr pivot arr i j hjr harltp ival hii hxi).1.val] pivot := by
+  induction ival, hii, hxi using hoare.classic.loop.while_i.induct (lt := lt) right hr pivot arr i j harltp with
   | case1 ival hii hxi hi hlt hir ih =>
     unfold hoare.classic.loop.while_i; simp [*]
   | case2 ival hii hxi hi hle =>
@@ -26,8 +27,8 @@ theorem hoare.classic.while_i_elem_not_left_of_piv {arr : Vector α n} {harltp :
 
 
 theorem hoare.classic.while_j_elem_not_right_of_piv {arr : Vector α n} {halgep : ¬lt pivot arr[left]} :
-  ¬lt pivot arr[(hoare.classic.loop.while_j left right hr hl pivot arr i j hjr hli halgep   jval hxj hjj).1.val] := by
-  induction jval, hxj, hjj using hoare.classic.loop.while_j.induct left right hr hl pivot arr i j hjr halgep with
+  ¬lt pivot arr[(hoare.classic.loop.while_j (lt := lt) left right hr hl pivot arr i j hjr hli halgep   jval hxj hjj).1.val] := by
+  induction jval, hxj, hjj using hoare.classic.loop.while_j.induct (lt := lt) left right hr hl pivot arr i j hjr halgep with
   | case1 jval hxj hjj hj hlt hjl ih =>
     unfold hoare.classic.loop.while_j; simp [*]
   | case2 jval hxj hjj hj  hle =>
@@ -37,8 +38,8 @@ theorem hoare.classic.while_j_elem_not_right_of_piv {arr : Vector α n} {halgep 
 
 
 theorem hoare.classic.while_i_before_is_left {arr : Vector α n} {harltp : ¬lt arr[right] pivot} :
-  RangeHas n (lt arr[·] pivot) ival (hoare.classic.loop.while_i left right hr pivot arr i j hjr harltp ival hii hxi) := by
-  induction ival, hii, hxi using hoare.classic.loop.while_i.induct right hr pivot arr i j harltp with
+  RangeHas n (lt arr[·] pivot) ival (hoare.classic.loop.while_i (lt := lt) left right hr pivot arr i j hjr harltp ival hii hxi) := by
+  induction ival, hii, hxi using hoare.classic.loop.while_i.induct (lt := lt) right hr pivot arr i j harltp with
   | case1 ival hii hxi hi hlt hir ih =>
     unfold hoare.classic.loop.while_i; simp [*]
     apply RangeHas.prepend <;> assumption
@@ -48,8 +49,8 @@ theorem hoare.classic.while_i_before_is_left {arr : Vector α n} {harltp : ¬lt 
 
 
 theorem hoare.classic.while_j_before_is_right {arr : Vector α n} {halgep : ¬lt pivot arr[left]} :
-  RangeHas n (lt pivot arr[·]) ((hoare.classic.loop.while_j left right hr hl pivot arr i j hjr hli halgep   jval hxj hjj) + 1) (jval + 1) := by
-  induction jval, hxj, hjj using hoare.classic.loop.while_j.induct left right hr hl pivot arr i j hjr halgep with
+  RangeHas n (lt pivot arr[·]) ((hoare.classic.loop.while_j (lt := lt) left right hr hl pivot arr i j hjr hli halgep   jval hxj hjj) + 1) (jval + 1) := by
+  induction jval, hxj, hjj using hoare.classic.loop.while_j.induct (lt := lt) left right hr hl pivot arr i j hjr halgep with
   | case1 jval hxj hjj hj hlt hjl ih =>
     unfold hoare.classic.loop.while_j; simp [*]
     replace ih := show (jval - 1 + 1) = jval by omega ▸ ih
@@ -59,7 +60,7 @@ theorem hoare.classic.while_j_before_is_right {arr : Vector α n} {halgep : ¬lt
     apply RangeHas.refl
 
 #check Partition.hoare.classic.loop.induct
-theorem hoare.classic.loop.partition_bounds {left right : Nat} {hr : right < n} {hl : left < n} {pivot : α} {arr : Vector α n} {i j : Nat} {hli : left < i} {hij : i ≤ j + 1} {hjr : j < right} {halgep : ¬lt pivot arr[left]} {harltp : ¬lt arr[right] pivot} : (loop left right hr hl pivot arr i j hli hij hjr halgep harltp).val.j' < (loop left right hr hl pivot arr i j hli hij hjr halgep harltp).val.i' := by
+theorem hoare.classic.loop.partition_bounds {left right : Nat} {hr : right < n} {hl : left < n} {pivot : α} {arr : Vector α n} {i j : Nat} {hli : left < i} {hij : i ≤ j + 1} {hjr : j < right} {halgep : ¬lt pivot arr[left]} {harltp : ¬lt arr[right] pivot} : (loop (lt := lt) left right hr hl pivot arr i j hli hij hjr halgep harltp).val.j' < (loop (lt := lt) left right hr hl pivot arr i j hli hij hjr halgep harltp).val.i' := by
   induction arr, i, j, hli, hij, hjr, halgep, harltp using loop.induct left right hr hl pivot; all_goals unfold loop; simp [*]
   · case  case1 arr i j hli hij hjr halgep harltp i' hi1' hi2' heq_i' j' hj' heq_j' hlt arr' halgep' harltp' ih =>
     -- unfold loop; simp [*]
@@ -71,7 +72,7 @@ theorem hoare.classic.loop.partition_bounds {left right : Nat} {hr : right < n} 
     -- unfold loop; simp [*] -- have hij : i' = j' := by omega
     omega
 
-theorem hoare.classic.loop.permStabilizing {left right : Nat} {hr : right < n} {hl : left < n} {pivot : α} {arr : Vector α n} {i j : Nat} {hli : left < i} {hij : i ≤ j + 1} {hjr : j < right} {halgep : ¬lt pivot arr[left]} {harltp : ¬lt arr[right] pivot} : PermStabilizing' i j (loop left right hr hl pivot arr i j hli hij hjr halgep harltp).val.arr' arr := by
+theorem hoare.classic.loop.permStabilizing {left right : Nat} {hr : right < n} {hl : left < n} {pivot : α} {arr : Vector α n} {i j : Nat} {hli : left < i} {hij : i ≤ j + 1} {hjr : j < right} {halgep : ¬lt pivot arr[left]} {harltp : ¬lt arr[right] pivot} : PermStabilizing' i j (loop (lt := lt) left right hr hl pivot arr i j hli hij hjr halgep harltp).val.arr' arr := by
   induction arr, i, j, hli, hij, hjr, halgep, harltp using loop.induct left right hr hl pivot; all_goals unfold loop; simp [*]
   · case case1 arr i j hli hij hjr halgep harltp i' hi1' hi2' heq_i' j' hj' heq_j' hlt arr' halgep' harltp' ih =>
     apply PermStabilizing'.trans
@@ -85,36 +86,36 @@ theorem hoare.classic.loop.permStabilizing {left right : Nat} {hr : right < n} {
 
 -- set_option trace.profiler true in
 include lt_asymm in
-theorem hoare.classic.loop.sorted {left right : Nat} {hr : right < n} {hl : left < n} {pivot : α} {arr : Vector α n} {i j : Nat} {hli : left < i} {hij : i ≤ j + 1} {hjr : j < right} {halgep : ¬lt pivot arr[left]} {harltp : ¬lt arr[right] pivot} : IsPartitioned i j pivot (loop left right hr hl pivot arr i j hli hij hjr halgep harltp).val := by
+theorem hoare.classic.loop.sorted {left right : Nat} {hr : right < n} {hl : left < n} {pivot : α} {arr : Vector α n} {i j : Nat} {hli : left < i} {hij : i ≤ j + 1} {hjr : j < right} {halgep : ¬lt pivot arr[left]} {harltp : ¬lt arr[right] pivot} : IsPartitioned (lt := lt) i j pivot (loop (lt := lt) left right hr hl pivot arr i j hli hij hjr halgep harltp).val := by
   induction arr, i, j, hli, hij, hjr, halgep, harltp using loop.induct left right hr hl pivot; all_goals unfold loop; simp [*]
   · case case1 arr i j hli hij hjr halgep harltp i' hi1' hi2' heq_i' j' hj' heq_j' hlt arr' halgep' harltp' ih =>
     constructor
     · refine RangeHas.trans ?_ ih.1
       intro k h1 h2
-      rw [loop.permStabilizing.2.1 k h2]; exact
+      rw [(loop.permStabilizing (lt := lt)).2.1 k h2]; exact
       if h : k = i' then by
         simp only [h, Fin.getElem_fin, arr.getElem_swap_left, show j' = _ from Subtype.ext_iff.1 heq_j'.symm]
-        exact hoare.classic.while_j_elem_not_right_of_piv
+        exact hoare.classic.while_j_elem_not_right_of_piv (lt := lt)
       else by
         have := show (arr.swap i' j')[k] = _ by
           apply arr.getElem_swap_of_ne; all_goals first | simp only ; omega | omega
         simp only [this]
         apply lt_asymm
         replace h2 : k < i' := by omega
-        apply hoare.classic.while_i_before_is_left k h1 ((show i' = _ from Subtype.ext_iff.1 heq_i'.symm) ▸ h2)
+        apply hoare.classic.while_i_before_is_left (lt := lt) k h1 ((show i' = _ from Subtype.ext_iff.1 heq_i'.symm) ▸ h2)
     · refine RangeHas.trans ih.2 ?_
       intro k h1 h2
-      rw [loop.permStabilizing.2.2 k h1]; exact
+      rw [(loop.permStabilizing  (lt := lt)).2.2 k h1]; exact
       if h : k = j' then by
         simp only [h, Fin.getElem_fin, arr.getElem_swap_right, show i' = _ from Subtype.ext_iff.1 heq_i'.symm]
-        exact hoare.classic.while_i_elem_not_left_of_piv
+        exact hoare.classic.while_i_elem_not_left_of_piv (lt := lt)
       else by
         have := show (arr.swap i' j')[k] = _ by
           apply arr.getElem_swap_of_ne; all_goals first | simp only ; omega | omega
         simp only [this]
         apply lt_asymm
         replace h1 : j' < k := by omega
-        apply hoare.classic.while_j_before_is_right k ((show j' = _ from Subtype.ext_iff.1 heq_j'.symm) ▸ h1) h2
+        apply hoare.classic.while_j_before_is_right (lt := lt) k ((show j' = _ from Subtype.ext_iff.1 heq_j'.symm) ▸ h1) h2
 
   · case case2 arr i j hli hij hjr halgep harltp i' hi1' hi2' heq_i' j' hj' heq_j' _ hlt' =>
     -- apply while_before_is_partitioned <;> assumption
@@ -122,11 +123,11 @@ theorem hoare.classic.loop.sorted {left right : Nat} {hr : right < n} {hl : left
     · intro k h1 h2
       apply lt_asymm
       have := show i' = _ from Subtype.ext_iff.1 heq_i'.symm
-      apply hoare.classic.while_i_before_is_left k h1 (this ▸ h2)
+      apply hoare.classic.while_i_before_is_left (lt := lt) k h1 (this ▸ h2)
     · intro k h1 h2
       apply lt_asymm
       have := show j' = _ from Subtype.ext_iff.1 heq_j'.symm
-      apply hoare.classic.while_j_before_is_right k (this ▸ h1) h2
+      apply hoare.classic.while_j_before_is_right (lt := lt) k (this ▸ h1) h2
 
   · case case3 arr i j hli hij hjr halgep harltp p_ hi1' hi2' heq_i' p hj' heq_j' _hij' _hij' =>
 
@@ -146,7 +147,7 @@ theorem hoare.classic.loop.sorted {left right : Nat} {hr : right < n} {hl : left
         intro k h1 h2
         apply lt_asymm
         have := show p = _ from Subtype.ext_iff.1 heq_i'.symm
-        apply while_i_before_is_left k h1 (this ▸ h2)
+        apply while_i_before_is_left (lt := lt) k h1 (this ▸ h2)
     · apply RangeHas.prepend
       · change ¬lt arr[p] pivot
         rw [show p = _ from Subtype.ext_iff.1 heq_i'.symm]
@@ -156,14 +157,14 @@ theorem hoare.classic.loop.sorted {left right : Nat} {hr : right < n} {hl : left
         intro k h1 h2
         apply lt_asymm
         have := show p = _ from Subtype.ext_iff.1 heq_j'.symm
-        apply hoare.classic.while_j_before_is_right k (this ▸ h1) h2
+        apply hoare.classic.while_j_before_is_right (lt := lt) k (this ▸ h1) h2
 
 -- -----------------------
 
 
 
 include lt_asymm in
-private theorem hoare.classic.sortAt_sorted (as : Vector α n) (low high : Nat) (hlh : low ≤ high) (hn : high < n) : ¬ (lt (maybeSwap as ⟨low, by omega⟩ ⟨high, by omega⟩)[high] (maybeSwap as ⟨low, by omega⟩ ⟨high, by omega⟩)[low]) := by
+private theorem hoare.classic.sortAt_sorted (as : Vector α n) (low high : Nat) (hlh : low ≤ high) (hn : high < n) : ¬ (lt (maybeSwap (lt := lt) as ⟨low, by omega⟩ ⟨high, by omega⟩)[high] (maybeSwap (lt := lt) as ⟨low, by omega⟩ ⟨high, by omega⟩)[low]) := by
   unfold maybeSwap; split
   · next h =>
       have _ := lt_asymm h
@@ -175,28 +176,28 @@ include lt_asymm in
 include le_trans in
 private theorem hoare.classic.median_of_three_sorted {arr : Vector α n} {left mid right: Nat} (hlm : left ≤ mid) (hmr : mid ≤ right) (hr : right < n) :
   have arr_ := arr
-    |> (maybeSwap · ⟨left, by omega⟩ ⟨mid, by omega⟩)
-    |> (maybeSwap · ⟨left, by omega⟩ ⟨right, by omega⟩)
-    |> (maybeSwap · ⟨mid, by omega⟩ ⟨right, by omega⟩)
+    |> (maybeSwap (lt := lt) · ⟨left, by omega⟩ ⟨mid, by omega⟩)
+    |> (maybeSwap (lt := lt) · ⟨left, by omega⟩ ⟨right, by omega⟩)
+    |> (maybeSwap (lt := lt) · ⟨mid, by omega⟩ ⟨right, by omega⟩)
 -- ∀ {k_ : Nat} (_ : left ≤ k_) (_ : k_ ≤ right),
   ¬lt arr_[mid] arr_[left] ∧ ¬lt arr_[right] arr_[mid]
   :=
   have _ : left < n := by omega
   have _ : mid < n := by omega
 
-  let arr1 : Vector α n := maybeSwap arr ⟨left, by omega⟩ ⟨mid, by omega⟩
-  let arr2 : Vector α n := maybeSwap arr1 ⟨left, by omega⟩ ⟨right, by omega⟩
-  let arr_ : Vector α n := maybeSwap arr2 ⟨mid, by omega⟩ ⟨right, by omega⟩
+  let arr1 : Vector α n := maybeSwap (lt := lt) arr ⟨left, by omega⟩ ⟨mid, by omega⟩
+  let arr2 : Vector α n := maybeSwap (lt := lt) arr1 ⟨left, by omega⟩ ⟨right, by omega⟩
+  let arr_ : Vector α n := maybeSwap (lt := lt) arr2 ⟨mid, by omega⟩ ⟨right, by omega⟩
 
-  have hh1 : ¬lt arr1[mid] arr1[left] := sortAt_sorted lt_asymm arr left mid (by omega) (by omega)
-  have hh2 : ¬lt arr2[right] arr2[left] := sortAt_sorted lt_asymm arr1 left right (by omega) (by omega)
-  have hh_ : ¬lt arr_[right] arr_[mid] := sortAt_sorted lt_asymm arr2 mid right (by omega) (by omega)
+  have hh1 : ¬lt arr1[mid] arr1[left] := sortAt_sorted (lt := lt) lt_asymm arr left mid (by omega) (by omega)
+  have hh2 : ¬lt arr2[right] arr2[left] := sortAt_sorted (lt := lt) lt_asymm arr1 left right (by omega) (by omega)
+  have hh_ : ¬lt arr_[right] arr_[mid] := sortAt_sorted (lt := lt) lt_asymm arr2 mid right (by omega) (by omega)
 
   suffices ¬lt arr_[mid] arr_[left] from ⟨this, hh_⟩
 
   if hleqm : left = mid then by
     simp only [hleqm]
-    exact lt_irrefl lt_asymm arr_[mid]
+    exact (lt_irrefl (lt := lt)) lt_asymm arr_[mid]
   else by
     have hlneqr : left ≠ right := by omega
     simp only [arr_]
@@ -225,16 +226,16 @@ private theorem hoare.classic.median_of_three_sorted {arr : Vector α n} {left m
 
 include le_trans in
 include lt_asymm in
-protected theorem hoare.classic.partition_bounds' {arr : Vector α n} {left : Nat} {right : Nat} {hlr : left < right} {hr : right < n} : (hoare.classic (lt_asymm := lt_asymm) (le_trans := le_trans) arr left right hlr hr).val.j' < (hoare.classic (lt_asymm := lt_asymm) (le_trans := le_trans) arr left right hlr hr).val.i' := by
+protected theorem hoare.classic.partition_bounds' {arr : Vector α n} {left : Nat} {right : Nat} {hlr : left < right} {hr : right < n} : (hoare.classic (lt := lt) (lt_asymm := lt_asymm) (le_trans := le_trans) arr left right hlr hr).val.j' < (hoare.classic (lt := lt) (lt_asymm := lt_asymm) (le_trans := le_trans) arr left right hlr hr).val.i' := by
   unfold hoare.classic
   apply Partition.hoare.classic.loop.partition_bounds
 
 
 include le_trans in
 include lt_asymm in
-protected theorem hoare.classic.permStabilizing' {arr : Vector α n} {left : Nat} {right : Nat} {hlr : left < right} {hr : right < n} : PermStabilizing' left right (hoare.classic (lt_asymm := lt_asymm) (le_trans := le_trans) arr left right hlr hr).val.arr' arr := by
+protected theorem hoare.classic.permStabilizing' {arr : Vector α n} {left : Nat} {right : Nat} {hlr : left < right} {hr : right < n} : PermStabilizing' left right (hoare.classic (lt := lt) (lt_asymm := lt_asymm) (le_trans := le_trans) arr left right hlr hr).val.arr' arr := by
   apply PermStabilizing'.trans
-  · apply PermStabilizing'.mono hoare.classic.loop.permStabilizing <;> omega
+  · apply PermStabilizing'.mono (hoare.classic.loop.permStabilizing  (lt := lt))  <;> omega
   · apply PermStabilizing'.trans
     apply PermStabilizing'.trans
     all_goals apply maybeSwap_permStabilizing
@@ -243,7 +244,7 @@ protected theorem hoare.classic.permStabilizing' {arr : Vector α n} {left : Nat
 
 include le_trans in
 include lt_asymm in
-protected theorem hoare.classic.sorted {arr : Vector α n} {left : Nat} {right : Nat} {hlr : left < right} {hr : right < n} : ∃ (pivot : α), IsPartitioned left right pivot (hoare.classic (lt_asymm := lt_asymm) (le_trans := le_trans) arr left right hlr hr).val :=
+protected theorem hoare.classic.sorted {arr : Vector α n} {left : Nat} {right : Nat} {hlr : left < right} {hr : right < n} : ∃ (pivot : α), IsPartitioned (lt := lt) left right pivot (hoare.classic  (lt := lt) (lt_asymm := lt_asymm) (le_trans := le_trans) arr left right hlr hr).val :=
 
   let mid := left + ((right - left)/2)
   have hlm : left ≤ mid := Nat.le_add_right left ((right - left) / 2)
@@ -255,18 +256,18 @@ protected theorem hoare.classic.sorted {arr : Vector α n} {left : Nat} {right :
   have hm :  mid < n := Trans.trans hmr hr
 
   let arr_ := arr
-    |> (maybeSwap · ⟨left, by omega⟩ ⟨mid, by omega⟩)
-    |> (maybeSwap · ⟨left, by omega⟩ ⟨right, by omega⟩)
-    |> (maybeSwap · ⟨mid, by omega⟩ ⟨right, by omega⟩)
+    |> (maybeSwap (lt := lt) · ⟨left, by omega⟩ ⟨mid, by omega⟩)
+    |> (maybeSwap (lt := lt) · ⟨left, by omega⟩ ⟨right, by omega⟩)
+    |> (maybeSwap (lt := lt) · ⟨mid, by omega⟩ ⟨right, by omega⟩)
   let pivot := arr_[mid]
 
-  have hh2 : ¬lt pivot arr_[left] ∧ ¬lt arr_[right] pivot := hoare.classic.median_of_three_sorted (lt_asymm := lt_asymm) (le_trans := le_trans) hlm hmr hr
-  let x : Partition α n := (hoare.classic.loop left right hr (by omega) pivot  arr_ (left + 1) (right - 1) (by omega) (by omega) (by omega) hh2.left hh2.right).val
+  have hh2 : ¬lt pivot arr_[left] ∧ ¬lt arr_[right] pivot := hoare.classic.median_of_three_sorted (lt := lt) (lt_asymm := lt_asymm) (le_trans := le_trans) hlm hmr hr
+  let x : Partition α n := (hoare.classic.loop (lt := lt) left right hr (by omega) pivot  arr_ (left + 1) (right - 1) (by omega) (by omega) (by omega) hh2.left hh2.right).val
 
-  have : IsPartitioned left right pivot x := by
-    have hh1 : IsPartitioned (left + 1) (right - 1) pivot x := hoare.classic.loop.sorted (lt_asymm := lt_asymm)
+  have : IsPartitioned (lt := lt) left right pivot x := by
+    have hh1 : IsPartitioned (lt := lt) (left + 1) (right - 1) pivot x := hoare.classic.loop.sorted (lt := lt) (lt_asymm := lt_asymm)
 
-    have : PermStabilizing' (left + 1) (right - 1) x.arr' arr_ := hoare.classic.loop.permStabilizing
+    have : PermStabilizing' (left + 1) (right - 1) x.arr' arr_ := hoare.classic.loop.permStabilizing (lt := lt)
     replace hh2 : ¬lt pivot x.arr'[left] ∧ ¬lt x.arr'[right] pivot := by
       have heq_left : x.arr'[left] = arr_[left] := this.2.1 ⟨left, by omega⟩ (by grind)
       have heq_right : x.arr'[right] = arr_[right] := this.2.2 ⟨right, by omega⟩ (by grind)
