Quicksort/Partition/Init/Lemmas.lean
@@ -4,9 +4,9 @@ import Quicksort.Partition.Init.Basic
 
 open Vector
 
-variable [Ord α]
+variable (lt : α → α → Bool := by exact (· < ·))
 
-theorem maybeSwap_permStabilizing {as : Vector α n} {i j : Fin n} {left right : Nat} (h_i1 : left ≤ i) (h_i2 : i ≤ right) (h_j1 : left ≤ j) (h_j2 : j ≤ right) : PermStabilizing' left right (as.maybeSwap i j) as := by
+theorem maybeSwap_permStabilizing {as : Vector α n} {i j : Fin n} {left right : Nat} (h_i1 : left ≤ i) (h_i2 : i ≤ right) (h_j1 : left ≤ j) (h_j2 : j ≤ right) : PermStabilizing' left right (as.maybeSwap (lt := lt) i j) as := by
   unfold maybeSwap
   split
   · apply swap_permStabilizing' <;> assumption
